LeanHoG/Invariant/HamiltonianCycle/Tactic.lean
@@ -36,7 +36,6 @@ unsafe def searchForHamiltonianCycleAux (graph : Q(Graph)) :
           | some true => cycle := cycle.set! j i
           | some false => continue
       let hpQ := hamiltonianCycleOfData graph ⟨cycle.toList⟩
-      IO.println s!"{cycle}"
       return some hpQ
     | .unsat =>
       -- TODO: Not yet implemented
@@ -50,13 +49,13 @@ unsafe def searchForHamiltonianCycleAux (graph : Q(Graph)) :
 -- Find Hamiltonian cycle command
 ------------------------------------------
 
-unsafe def checkHamiltonianCycleAux (graphName : Name) (graph : Q(Graph)) : TermElabM Unit := do
+unsafe def checkHamiltonianCycleAux (graphName : Name) (graph : Q(Graph)) : TermElabM Bool := do
   -- Check if there already exists an instance of a Hamiltonian cycle for g
   let inst ← Qq.trySynthInstanceQ q(HamiltonianCycle $graph)
   match inst with
   | .some _ =>
     logInfo "Hamiltonian cycle found"
-    pure ()
+    return true
   | _ =>
     let hpQOpt ← searchForHamiltonianCycleAux graph
     match hpQOpt with
@@ -72,8 +71,10 @@ unsafe def checkHamiltonianCycleAux (graphName : Name) (graph : Q(Graph)) : Term
       }
       Lean.Meta.addInstance hamiltonianCycleName .scoped 42
       logInfo "Hamiltonian cycle found"
+      return true
     | none =>
       logWarning s!"Hamiltonian cycle not found after exhaustive search"
+      return false
 
 syntax (name := checkHamiltonian) "#check_hamiltonian " ident : command
 /-- `#check_hamiltonian G` runs a SAT solver on the encoding of the Hamiltonian cycle problem
@@ -86,7 +87,7 @@ unsafe def checkHamiltonianImpl : Command.CommandElab
   | `(#check_hamiltonian $g) => Command.liftTermElabM do
     let graphName := g.getId
     let graph ← Qq.elabTermEnsuringTypeQ g q(Graph)
-    checkHamiltonianCycleAux graphName graph
+    let _ ← checkHamiltonianCycleAux graphName graph
 
   | _ => throwUnsupportedSyntax
 
@@ -94,6 +95,19 @@ unsafe def checkHamiltonianImpl : Command.CommandElab
 -- Find Hamiltonian cycle tactic
 ------------------------------------------
 -- TODO: Remove code duplication once I figure out how to do it corectly.
+
+unsafe def checkHamiltonianTacticAux (graphName : Name) (graph : Q(Graph)) (hypName : Name) :
+  Tactic.TacticM Unit := do
+  let isHamiltonian ← checkHamiltonianCycleAux graphName graph
+  if isHamiltonian then
+    let existsHamPath ← Meta.mkAppM ``LeanHoG.HamiltonianPath.path_of_cert #[]
+    let existsType := q(Graph.traceable $graph)
+    Tactic.liftMetaTactic fun mvarId => do
+      let mvarIdNew ← mvarId.assert hypName existsHamPath existsType
+      let (_, mvarIdNew) ← mvarIdNew.intro1P
+      return [mvarIdNew]
+  else
+    throwError "cannot prove non-Hamiltonicity, not implemented!"
 
 syntax (name := checkHamiltonianTactic) "check_hamiltonian " ident (" with" (ppSpace colGt ident))? : tactic
 open LeanSAT Model in
@@ -110,7 +124,13 @@ unsafe def checkHamiltonianTacticImpl : Tactic.Tactic
     Tactic.withMainContext do
       let graphName := g.getId
       let graph ← Qq.elabTermEnsuringTypeQ g q(Graph)
-      checkHamiltonianCycleAux graphName graph
+      checkHamiltonianTacticAux graphName graph .anonymous
+
+  | `(tactic|check_hamiltonian $g with $h) =>
+    Tactic.withMainContext do
+      let graphName := g.getId
+      let graph ← Qq.elabTermEnsuringTypeQ g q(Graph)
+      checkHamiltonianTacticAux graphName graph h.getId
 
   | _ => throwUnsupportedSyntax
 
